theories/ml_toy_lang/melocoton/primitive_laws.v
@@ -12,8 +12,8 @@ From iris.prelude Require Import options.
 
 Class heapGS_gen hlc Σ := HeapGS {
   heapGS_invGS : invGS_gen hlc Σ;
-  heapGS_gen_heapGS :> gen_heapGS loc val Σ;
-  heapGS_inv_heapGS :> inv_heapGS loc val Σ;
+  heapGS_gen_heapGS :> gen_heapGS loc (list val) Σ;
+  heapGS_inv_heapGS :> inv_heapGS loc (list val) Σ;
   heapGS_step_name : gname;
   heapGS_step_cnt : mono_natG Σ;
 }.
@@ -59,7 +59,7 @@ Section steps.
 End steps.
 
 
-Global Program Instance heapGS_melocotonGS `{heapGS_gen hlc Σ} 
+Global Program Instance heapGS_melocotonGS `{heapGS_gen hlc Σ}
       : melocotonGS_gen hlc val ML_lang Σ := {
   iris_invGS := heapGS_invGS;
   state_interp σ step_cnt :=
@@ -70,53 +70,59 @@ Next Obligation.
   by iMod (steps_auth_update_S with "H") as "$".
 Qed.
 
-(** Since we use an [val] instance of [gen_heap], we need to overwrite
-the notations.  That also helps for scopes and coercions. *)
-(** FIXME: Refactor these notations using custom entries once Coq bug #13654
-has been fixed. *)
-Notation "l ↦{ dq } v" := (mapsto (L:=loc) (V:=val) l dq (v%V))
+Notation "l ↦{ dq } v" := (mapsto (L:=loc) (V:=list val) l dq [v%V])
   (at level 20, format "l  ↦{ dq }  v") : bi_scope.
-Notation "l ↦□ v" := (mapsto (L:=loc) (V:=val) l DfracDiscarded (v%V))
+Notation "l ↦□ v" := (mapsto (L:=loc) (V:=list val) l DfracDiscarded [v%V])
   (at level 20, format "l  ↦□  v") : bi_scope.
-Notation "l ↦{# q } v" := (mapsto (L:=loc) (V:=val) l (DfracOwn q) (v%V))
+Notation "l ↦{# q } v" := (mapsto (L:=loc) (V:=list val) l (DfracOwn q) [v%V])
   (at level 20, format "l  ↦{# q }  v") : bi_scope.
-Notation "l ↦ v" := (mapsto (L:=loc) (V:=val) l (DfracOwn 1) (v%V))
+Notation "l ↦ v" := (mapsto (L:=loc) (V:=list val) l (DfracOwn 1) [v%V])
   (at level 20, format "l  ↦  v") : bi_scope.
+
+Notation "l ↦∗{ dq } vs" := (mapsto (L:=loc) (V:=list val) l dq vs)
+  (at level 20, format "l  ↦∗{ dq }  vs") : bi_scope.
+Notation "l ↦∗□ vs" := (mapsto (L:=loc) (V:=list val) l DfracDiscarded vs)
+  (at level 20, format "l  ↦∗□  vs") : bi_scope.
+Notation "l ↦∗{# q } vs" := (mapsto (L:=loc) (V:=list val) l (DfracOwn q) vs)
+  (at level 20, format "l  ↦∗{# q }  vs") : bi_scope.
+Notation "l ↦∗ vs" := (mapsto (L:=loc) (V:=list val) l (DfracOwn 1) vs)
+  (at level 20, format "l  ↦∗  vs") : bi_scope.
 
 (** Same for [gen_inv_heap], except that these are higher-order notations so to
 make setoid rewriting in the predicate [I] work we need actual definitions
 here. *)
 Section definitions.
   Context `{!heapGS_gen hlc Σ}.
-  Definition inv_mapsto_own (l : loc) (v : val) (I : val → Prop) : iProp Σ :=
-    inv_mapsto_own l v I.
-  Definition inv_mapsto (l : loc) (I : val → Prop) : iProp Σ :=
+  Definition inv_mapsto_own (l : loc) (vs : list val) (I : list val → Prop) : iProp Σ :=
+    inv_mapsto_own l vs I.
+  Definition inv_mapsto (l : loc) (I : list val → Prop) : iProp Σ :=
     inv_mapsto l I.
+  (* TODO: single value version of those *)
 End definitions.
 
 Global Instance: Params (@inv_mapsto_own) 4 := {}.
 Global Instance: Params (@inv_mapsto) 3 := {}.
 
-Notation inv_heap_inv := (inv_heap_inv loc val).
-Notation "l '↦_' I □" := (inv_mapsto l I%stdpp%type)
-  (at level 20, I at level 9, format "l  '↦_' I  '□'") : bi_scope.
-Notation "l ↦_ I v" := (inv_mapsto_own l v I%stdpp%type)
-  (at level 20, I at level 9, format "l  ↦_ I  v") : bi_scope.
+Notation inv_heap_inv := (inv_heap_inv loc (list val)).
+Notation "l '↦∗_' I □" := (inv_mapsto l I%stdpp%type)
+  (at level 20, I at level 9, format "l  '↦∗_' I  '□'") : bi_scope.
+Notation "l ↦∗_ I vs" := (inv_mapsto_own l vs I%stdpp%type)
+  (at level 20, I at level 9, format "l  ↦∗_ I  vs") : bi_scope.
 
 Section lifting.
 Context `{!heapGS_gen hlc Σ}.
 Implicit Types P Q : iProp Σ.
 Implicit Types Φ Ψ : val → iProp Σ.
-Implicit Types efs : list expr.
 Implicit Types σ : state.
 Implicit Types v : val.
+Implicit Types vs : list val.
 Implicit Types l : loc.
-Implicit Types s : prog_environ ML_lang Σ.
+Implicit Types pe : prog_environ ML_lang Σ.
 
-Lemma wp_lb_init s E e Φ :
+Lemma wp_lb_init pe E e Φ :
   TCEq (to_val e) None →
-  (steps_lb 0 -∗ WP e @ s; E {{ v, Φ v }}) -∗
-  WP e @ s; E {{ Φ }}.
+  (steps_lb 0 -∗ WP e @ pe; E {{ v, Φ v }}) -∗
+  WP e @ pe; E {{ Φ }}.
 Proof.
   (** TODO: We should try to use a generic lifting lemma (and avoid [wp_unfold])
   here, since this breaks the WP abstraction. *)
@@ -127,11 +133,11 @@ Proof.
   iSpecialize ("Hwp" with "Hlb0"). iApply ("Hwp" $! σ1 ns). iFrame.
 Qed.
 
-Lemma wp_lb_update s n E e Φ :
+Lemma wp_lb_update pe n E e Φ :
   TCEq (to_val e) None →
   steps_lb n -∗
-  WP e @ s; E {{ v, steps_lb n -∗ Φ v }} -∗
-  WP e @ s; E {{ Φ }}.
+  WP e @ pe; E {{ v, steps_lb n -∗ Φ v }} -∗
+  WP e @ pe; E {{ Φ }}.
 Proof.
   (** TODO: We should try to use a generic lifting lemma (and avoid [wp_unfold])
   here, since this breaks the WP abstraction. *)
@@ -159,10 +165,10 @@ Qed.
 (** Recursive functions: we do not use this lemmas as it is easier to use Löb
 induction directly, but this demonstrates that we can state the expected
 reasoning principle for recursive functions, without any visible ▷. *)
-Lemma wp_rec_löb s E f x e Φ Ψ :
-  □ ( □ (∀ v, Ψ v -∗ WP (rec: f x := e)%V v @ s; E {{ Φ }}) -∗
-     ∀ v, Ψ v -∗ WP (subst' x v (subst' f (rec: f x := e) e)) @ s; E {{ Φ }}) -∗
-  ∀ v, Ψ v -∗ WP (rec: f x := e)%V v @ s; E {{ Φ }}.
+Lemma wp_rec_löb pe E f x e Φ Ψ :
+  □ ( □ (∀ v, Ψ v -∗ WP (rec: f x := e)%V v @ pe; E {{ Φ }}) -∗
+     ∀ v, Ψ v -∗ WP (subst' x v (subst' f (rec: f x := e) e)) @ pe; E {{ Φ }}) -∗
+  ∀ v, Ψ v -∗ WP (rec: f x := e)%V v @ pe; E {{ Φ }}.
 Proof.
   iIntros "#Hrec". iLöb as "IH". iIntros (v) "HΨ".
   iApply lifting.wp_pure_step_later; first eauto.
@@ -201,8 +207,8 @@ Proof. apply mapsto_ne. Qed.
 Lemma mapsto_persist l dq v : l ↦{dq} v ==∗ l ↦□ v.
 Proof. apply mapsto_persist. Qed.
 
-Global Instance inv_mapsto_own_proper l v :
-  Proper (pointwise_relation _ iff ==> (≡)) (inv_mapsto_own l v).
+Global Instance inv_mapsto_own_proper l vs :
+  Proper (pointwise_relation _ iff ==> (≡)) (inv_mapsto_own l vs).
 Proof.
   intros I1 I2 HI. rewrite /inv_mapsto_own. f_equiv; done.
 Qed.
@@ -212,19 +218,19 @@ Proof.
   intros I1 I2 HI. rewrite /inv_mapsto. f_equiv; done.
 Qed.
 
-Lemma make_inv_mapsto l v (I : val → Prop) E :
+Lemma make_inv_mapsto l vs (I : list val → Prop) E :
   ↑inv_heapN ⊆ E →
-  I v →
-  inv_heap_inv -∗ l ↦ v ={E}=∗ l ↦_I v.
+  I vs →
+  inv_heap_inv -∗ l ↦∗ vs ={E}=∗ l ↦∗_I vs.
 Proof. iIntros (??) "#HI Hl". iApply make_inv_mapsto; done. Qed.
-Lemma inv_mapsto_own_inv l v I : l ↦_I v -∗ l ↦_I □.
+Lemma inv_mapsto_own_inv l vs I : l ↦∗_I vs -∗ l ↦∗_I □.
 Proof. apply inv_mapsto_own_inv. Qed.
 
 Lemma inv_mapsto_own_acc_strong E :
   ↑inv_heapN ⊆ E →
-  inv_heap_inv ={E, E ∖ ↑inv_heapN}=∗ ∀ l v I, l ↦_I v -∗
-    (⌜I v⌝ ∗ l ↦ v ∗ (∀ w, ⌜I w ⌝ -∗ l ↦ w ==∗
-      inv_mapsto_own l w I ∗ |={E ∖ ↑inv_heapN, E}=> True)).
+  inv_heap_inv ={E, E ∖ ↑inv_heapN}=∗ ∀ l vs I, l ↦∗_I vs -∗
+    (⌜I vs⌝ ∗ l ↦∗ vs ∗ (∀ ws, ⌜I ws⌝ -∗ l ↦∗ ws ==∗
+      inv_mapsto_own l ws I ∗ |={E ∖ ↑inv_heapN, E}=> True)).
 Proof.
   iIntros (?) "#Hinv".
   iMod (inv_mapsto_own_acc_strong with "Hinv") as "Hacc"; first done.
@@ -232,10 +238,10 @@ Proof.
   iFrame "%∗".
 Qed.
 
-Lemma inv_mapsto_own_acc E l v I:
+Lemma inv_mapsto_own_acc E l vs I:
   ↑inv_heapN ⊆ E →
-  inv_heap_inv -∗ l ↦_I v ={E, E ∖ ↑inv_heapN}=∗
-    (⌜I v⌝ ∗ l ↦ v ∗ (∀ w, ⌜I w ⌝ -∗ l ↦ w ={E ∖ ↑inv_heapN, E}=∗ l ↦_I w)).
+  inv_heap_inv -∗ l ↦∗_I vs ={E, E ∖ ↑inv_heapN}=∗
+    (⌜I vs⌝ ∗ l ↦∗ vs ∗ (∀ ws, ⌜I ws ⌝ -∗ l ↦∗ ws ={E ∖ ↑inv_heapN, E}=∗ l ↦∗_I ws)).
 Proof.
   iIntros (?) "#Hinv Hl".
   iMod (inv_mapsto_own_acc with "Hinv Hl") as "(% & Hl & Hclose)"; first done.
@@ -244,220 +250,97 @@ Qed.
 
 Lemma inv_mapsto_acc l I E :
   ↑inv_heapN ⊆ E →
-  inv_heap_inv -∗ l ↦_I □ ={E, E ∖ ↑inv_heapN}=∗
-    ∃ v, ⌜I v⌝ ∗ l ↦ v ∗ (l ↦ v ={E ∖ ↑inv_heapN, E}=∗ ⌜True⌝).
+  inv_heap_inv -∗ l ↦∗_I □ ={E, E ∖ ↑inv_heapN}=∗
+    ∃ vs, ⌜I vs⌝ ∗ l ↦∗ vs ∗ (l ↦∗ vs ={E ∖ ↑inv_heapN, E}=∗ ⌜True⌝).
 Proof.
   iIntros (?) "#Hinv Hl".
   iMod (inv_mapsto_acc with "Hinv Hl") as (v) "(% & Hl & Hclose)"; [done|].
   iIntros "!>". iExists (v). iFrame "%∗".
 Qed.
 
-(** The usable rules for [allocN] stated in terms of the [array] proposition
-are derived in te file [array]. *)
-Lemma heap_array_to_seq_meta l vs (n : nat) :
-  length vs = n →
-  ([∗ map] l' ↦ _ ∈ heap_array l vs, meta_token l' ⊤) -∗
-  [∗ list] i ∈ seq 0 n, meta_token (l +ₗ (i : nat)) ⊤.
-Proof.
-  iIntros (<-) "Hvs". iInduction vs as [|v vs] "IH" forall (l)=> //=.
-  rewrite big_opM_union; last first.
-  { apply map_disjoint_spec=> l' v1 v2 /lookup_singleton_Some [-> _].
-    intros (j&w&Hjl&?)%heap_array_lookup.
-    rewrite loc_add_assoc -{1}[l']loc_add_0 in Hjl. simplify_eq; lia. }
-  rewrite loc_add_0 -fmap_S_seq big_sepL_fmap.
-  setoid_rewrite Nat2Z.inj_succ. setoid_rewrite <-Z.add_1_l.
-  setoid_rewrite <-loc_add_assoc.
-  rewrite big_opM_singleton; iDestruct "Hvs" as "[$ Hvs]". by iApply "IH".
-Qed.
-
-Lemma heap_array_to_seq_mapsto l v (n : nat) :
-  ([∗ map] l' ↦ ov ∈ heap_array l (replicate n v), gen_heap.mapsto l' (DfracOwn 1) ov) -∗
-  [∗ list] i ∈ seq 0 n, (l +ₗ (i : nat)) ↦ v.
-Proof.
-  iIntros "Hvs". iInduction n as [|n] "IH" forall (l); simpl.
-  { done. }
-  rewrite big_opM_union; last first.
-  { apply map_disjoint_spec=> l' v1 v2 /lookup_singleton_Some [-> _].
-    intros (j&w&Hjl&_)%heap_array_lookup.
-    rewrite loc_add_assoc -{1}[l']loc_add_0 in Hjl. simplify_eq; lia. }
-  rewrite loc_add_0 -fmap_S_seq big_sepL_fmap.
-  setoid_rewrite Nat2Z.inj_succ. setoid_rewrite <-Z.add_1_l.
-  setoid_rewrite <-loc_add_assoc.
-  rewrite big_opM_singleton; iDestruct "Hvs" as "[$ Hvs]". by iApply "IH".
-Qed.
-
-Lemma wp_allocN_seq s E v n :
-  (0 < n)%Z →
-  {{{ True }}} AllocN (Val $ LitV $ LitInt $ n) (Val v) @ s; E
-  {{{ l, RET LitV (LitLoc l); [∗ list] i ∈ seq 0 (Z.to_nat n),
-      (l +ₗ (i : nat)) ↦ v ∗ meta_token (l +ₗ (i : nat)) ⊤ }}}.
+Lemma wp_allocN pe E v n :
+  (0 ≤ n)%Z →
+  {{{ True }}} AllocN (Val $ LitV $ LitInt n) (Val v) @ pe; E
+  {{{ l, RET LitV (LitLoc l); l ↦∗ (replicate (Z.to_nat n) v) ∗ meta_token l ⊤ }}}.
 Proof.
   iIntros (Hn Φ) "_ HΦ". iApply wp_lift_atomic_head_step; first done.
-  iIntros (σ1 ns) "(Hσ & Hsteps)". iModIntro. iSplit; first (destruct n; eauto with lia head_step).  
+  iIntros (σ1 ns) "(Hσ & Hsteps)". iModIntro. iSplit; first (destruct n; eauto with lia head_step).
   iIntros (v2 σ2 Hstep). inv_head_step. iModIntro.
-  iMod (gen_heap_alloc_big _ (heap_array _ (replicate (Z.to_nat n) v)) with "Hσ")
-    as "(Hσ & Hl & Hm)".
-  { apply heap_array_map_disjoint.
-    rewrite replicate_length Z2Nat.id; auto with lia. }
+  iMod (gen_heap_alloc _ l (replicate (Z.to_nat n) v) with "Hσ") as "(Hσ & Hl & Hm)".
+  { by apply not_elem_of_dom. }
   iMod (steps_auth_update_S with "Hsteps") as "Hsteps".
-  iModIntro. iFrame. iApply "HΦ".
-  iApply big_sepL_sep. iSplitL "Hl".
-  - by iApply heap_array_to_seq_mapsto.
-  - iApply (heap_array_to_seq_meta with "Hm"). by rewrite replicate_length.
+  iModIntro. iFrame. iApply "HΦ". by iFrame.
 Qed.
 
-Lemma wp_alloc s E v :
-  {{{ True }}} Alloc (Val v) @ s; E {{{ l, RET LitV (LitLoc l); l ↦ v ∗ meta_token l ⊤ }}}.
+Lemma wp_alloc pe E v :
+  {{{ True }}} Alloc (Val v) @ pe; E
+  {{{ l, RET LitV (LitLoc l); l ↦ v ∗ meta_token l ⊤ }}}.
 Proof.
-  iIntros (Φ) "_ HΦ". iApply wp_allocN_seq; [auto with lia..|]. iModIntro.
-  iIntros (l) "/= (? & _)". rewrite loc_add_0. iApply "HΦ"; iFrame.
+  iIntros (HΦ) "_ HΦ". by iApply wp_allocN.
 Qed.
 
-(*
-Lemma swp_free s E l v :
-  {{{ l ↦ v }}} Free (Val $ LitV $ LitLoc l) @ s; E
-  {{{ RET LitV LitUnit; True }}}.
+Lemma wp_loadN pe E l i dq vs v :
+  (0 ≤ i)%Z →
+  vs !! Z.to_nat i = Some v →
+  {{{ ▷ l ↦∗{dq} vs }}} LoadN (Val $ LitV $ LitLoc l) (Val $ LitV $ LitInt i) @ pe; E
+  {{{ RET v; l ↦∗{dq} vs }}}.
 Proof.
-  iIntros (Φ) "Hl HΦ". iApply twp_lift_atomic_head_step_no_fork; first done.
-  iIntros (σ1 ns κs nt) "(Hσ & Hsteps) !>". iDestruct (gen_heap_valid with "Hσ Hl") as %?.
-  iSplit; first by eauto with head_step.
-  iIntros (κ v2 σ2 efs Hstep); inv_head_step.
-  iMod (gen_heap_update with "Hσ Hl") as "[$ Hl]".
-  iMod (steps_auth_update_S with "Hsteps") as "Hsteps".
-  iModIntro. iSplit; first done. iSplit; first done. iFrame. by iApply "HΦ".
-Qed.
-Lemma wp_free s E l v :
-  {{{ ▷ l ↦ v }}} Free (Val $ LitV (LitLoc l)) @ s; E
-  {{{ RET LitV LitUnit; True }}}.
-Proof.
-  iIntros (Φ) ">H HΦ". iApply (twp_wp_step with "HΦ").
-  iApply (twp_free with "H"); [by auto..|]; iIntros "H HΦ". by iApply "HΦ".
-Qed. *)
-
-Lemma wp_load' s E l dq v :
-  {{{ l ↦{dq} v }}} Load (Val $ LitV $ LitLoc l) @ s; E {{{ RET v; l ↦{dq} v }}}.
-Proof.
-  iIntros (Φ) "Hl HΦ". iApply wp_lift_atomic_head_step; first done.
+  iIntros (Hi Hv Φ) ">Hl HΦ". iApply wp_lift_atomic_head_step; first done.
   iIntros (σ1 ns) "(Hσ & Hsteps) !>". iDestruct (gen_heap_valid with "Hσ Hl") as %?.
-  iSplit; first by eauto with head_step. iModIntro.
-  iIntros (v2 σ2 Hstep); inv_head_step.
+  assert (σ1 !! l.[i] = Some v).
+  { rewrite store_lookup_eq. case_bool_decide; [|done]. by simplify_map_eq/=. }
+  iSplit; first by eauto with head_step.
+  iIntros (v2 σ2 Hstep); inv_head_step. iModIntro.
   iMod (steps_auth_update_S with "Hsteps") as "Hsteps". iFrame.
   by iApply "HΦ".
 Qed.
-Lemma wp_load s E l dq v :
-  {{{ ▷ l ↦{dq} v }}} Load (Val $ LitV $ LitLoc l) @ s; E {{{ RET v; l ↦{dq} v }}}.
+
+Lemma wp_load pe E l dq v :
+  {{{ ▷ l ↦{dq} v }}} Load (Val $ LitV $ LitLoc l) @ pe; E
+  {{{ RET v; l ↦{dq} v }}}.
 Proof.
-  iIntros (Φ) ">Hl HΦ". iApply (wp_step with "HΦ").
-  iApply (wp_load' with "Hl"). iIntros "!> H HΦ". by iApply "HΦ".
+  iIntros (Φ) ">Hl HΦ". by iApply (wp_loadN with "Hl").
 Qed.
 
-Lemma wp_store' s E l v' v :
-  {{{ l ↦ v' }}} Store (Val $ LitV $ LitLoc l) (Val v) @ s; E
-  {{{ RET LitV LitUnit; l ↦ v }}}.
+Lemma wp_storeN pe E l i vs w :
+  (0 ≤ i < length vs)%Z →
+  {{{ ▷ l ↦∗ vs }}} StoreN (Val $ LitV $ LitLoc l) (Val $ LitV $ LitInt i) (Val w) @ pe; E
+  {{{ RET LitV LitUnit; l ↦∗ <[ Z.to_nat i := w ]> vs }}}.
 Proof.
-  iIntros (Φ) "Hl HΦ". iApply wp_lift_atomic_head_step; first done.
+  iIntros (Hi Φ) ">Hl HΦ". iApply wp_lift_atomic_head_step; first done.
+  iIntros (σ1 ns) "(Hσ & Hsteps) !>". iDestruct (gen_heap_valid with "Hσ Hl") as %?.
+  assert (is_Some (σ1 !! l.[i])) as [? ?].
+  { rewrite store_lookup_eq. case_bool_decide; [|lia]. simplify_map_eq.
+    apply lookup_lt_is_Some. lia. }
+  iSplit; first by eauto with head_step.
+  iIntros (v2 σ2 Hstep); inv_head_step. iModIntro.
+  iMod (steps_auth_update_S with "Hsteps") as "Hsteps".
+  iMod (gen_heap_update with "Hσ Hl") as "[Hσ Hl]".
+  rewrite (store_insert_offset _ _ _ vs); auto; [].
+  iFrame "Hσ Hsteps". by iApply "HΦ".
+Qed.
+
+Lemma wp_store pe E l v w :
+  {{{ ▷ l ↦ v }}} Store (Val $ LitV $ LitLoc l) (Val w) @ pe; E
+  {{{ RET LitV LitUnit; l ↦ w }}}.
+Proof.
+  iIntros (Φ) "Hl HΦ". by iApply (wp_storeN with "Hl").
+Qed.
+
+Lemma wp_length pe E l dq vs :
+  {{{ ▷ l ↦∗{dq} vs }}} Length (Val $ LitV $ LitLoc l) @ pe; E
+  {{{ RET LitV $ LitInt (length vs); l ↦∗{dq} vs }}}.
+Proof.
+  iIntros (Φ) ">Hl HΦ". iApply wp_lift_atomic_head_step; first done.
   iIntros (σ1 ns) "(Hσ & Hsteps) !>". iDestruct (gen_heap_valid with "Hσ Hl") as %?.
   iSplit; first by eauto with head_step.
   iIntros (v2 σ2 Hstep); inv_head_step. iModIntro.
   iMod (steps_auth_update_S with "Hsteps") as "Hsteps".
-  iMod (gen_heap_update with "Hσ Hl") as "[$ Hl]".
-  iModIntro. iFrame. by iApply "HΦ".
-Qed.
-Lemma wp_store s E l v' v :
-  {{{ ▷ l ↦ v' }}} Store (Val $ LitV (LitLoc l)) (Val v) @ s; E
-  {{{ RET LitV LitUnit; l ↦ v }}}.
-Proof.
-  iIntros (Φ) ">H HΦ". iApply (wp_step with "HΦ").
-  iApply (wp_store' with "H"). iIntros "!> H HΦ". by iApply "HΦ".
+  iFrame. by iApply "HΦ".
 Qed.
 
-
-
-
-(*
-Lemma twp_xchg s E l v' v :
-  {{{ l ↦ v' }}} Xchg (Val $ LitV $ LitLoc l) (Val v) @ s; E
-  {{{ RET v'; l ↦ v }}}.
-Proof.
-  iIntros (Φ) "Hl HΦ". iApply twp_lift_atomic_head_step_no_fork; first done.
-  iIntros (σ1 ns κs nt) "(Hσ & Hκs & Hsteps) !>". iDestruct (gen_heap_valid with "Hσ Hl") as %?.
-  iSplit; first by eauto with head_step.
-  iIntros (κ v2 σ2 efs Hstep); inv_head_step.
-  iMod (steps_auth_update_S with "Hsteps") as "Hsteps".
-  iMod (gen_heap_update with "Hσ Hl") as "[$ Hl]".
-  iModIntro. iSplit; first done. iSplit; first done. iFrame. by iApply "HΦ".
-Qed.
-Lemma wp_xchg s E l v' v :
-  {{{ ▷ l ↦ v' }}} Xchg (Val $ LitV (LitLoc l)) (Val v) @ s; E
-  {{{ RET v'; l ↦ v }}}.
-Proof.
-  iIntros (Φ) ">H HΦ". iApply (twp_wp_step with "HΦ").
-  iApply (twp_xchg with "H"); [by auto..|]. iIntros "H HΦ". by iApply "HΦ".
-Qed.
-
-Lemma twp_cmpxchg_fail s E l dq v' v1 v2 :
-  v' ≠ v1 → vals_compare_safe v' v1 →
-  {{{ l ↦{dq} v' }}} CmpXchg (Val $ LitV $ LitLoc l) (Val v1) (Val v2) @ s; E
-  {{{ RET PairV v' (LitV $ LitBool false); l ↦{dq} v' }}}.
-Proof.
-  iIntros (?? Φ) "Hl HΦ". iApply twp_lift_atomic_head_step_no_fork; first done.
-  iIntros (σ1 ns κs nt) "(Hσ & Hκs & Hsteps) !>". iDestruct (gen_heap_valid with "Hσ Hl") as %?.
-  iSplit; first by eauto with head_step.
-  iIntros (κ v2' σ2 efs Hstep); inv_head_step.
-  rewrite bool_decide_false //.
-  iMod (steps_auth_update_S with "Hsteps") as "Hsteps".
-  iModIntro; iSplit; first done. iSplit; first done. iFrame. by iApply "HΦ".
-Qed.
-Lemma wp_cmpxchg_fail s E l dq v' v1 v2 :
-  v' ≠ v1 → vals_compare_safe v' v1 →
-  {{{ ▷ l ↦{dq} v' }}} CmpXchg (Val $ LitV $ LitLoc l) (Val v1) (Val v2) @ s; E
-  {{{ RET PairV v' (LitV $ LitBool false); l ↦{dq} v' }}}.
-Proof.
-  iIntros (?? Φ) ">H HΦ". iApply (twp_wp_step with "HΦ").
-  iApply (twp_cmpxchg_fail with "H"); [by auto..|]; iIntros "H HΦ". by iApply "HΦ".
-Qed.
-
-Lemma twp_cmpxchg_suc s E l v1 v2 v' :
-  v' = v1 → vals_compare_safe v' v1 →
-  {{{ l ↦ v' }}} CmpXchg (Val $ LitV $ LitLoc l) (Val v1) (Val v2) @ s; E
-  {{{ RET PairV v' (LitV $ LitBool true); l ↦ v2 }}}.
-Proof.
-  iIntros (?? Φ) "Hl HΦ". iApply twp_lift_atomic_head_step_no_fork; first done.
-  iIntros (σ1 ns κs nt) "(Hσ & Hκs & Hsteps) !>". iDestruct (gen_heap_valid with "Hσ Hl") as %?.
-  iSplit; first by eauto with head_step.
-  iIntros (κ v2' σ2 efs Hstep); inv_head_step.
-  rewrite bool_decide_true //.
-  iMod (gen_heap_update with "Hσ Hl") as "[$ Hl]".
-  iMod (steps_auth_update_S with "Hsteps") as "Hsteps".
-  iModIntro. iSplit; first done. iSplit; first done. iFrame. by iApply "HΦ".
-Qed.
-Lemma wp_cmpxchg_suc s E l v1 v2 v' :
-  v' = v1 → vals_compare_safe v' v1 →
-  {{{ ▷ l ↦ v' }}} CmpXchg (Val $ LitV $ LitLoc l) (Val v1) (Val v2) @ s; E
-  {{{ RET PairV v' (LitV $ LitBool true); l ↦ v2 }}}.
-Proof.
-  iIntros (?? Φ) ">H HΦ". iApply (twp_wp_step with "HΦ").
-  iApply (twp_cmpxchg_suc with "H"); [by auto..|]; iIntros "H HΦ". by iApply "HΦ".
-Qed.
-
-Lemma twp_faa s E l i1 i2 :
-  {{{ l ↦ LitV (LitInt i1) }}} FAA (Val $ LitV $ LitLoc l) (Val $ LitV $ LitInt i2) @ s; E
-  {{{ RET LitV (LitInt i1); l ↦ LitV (LitInt (i1 + i2)) }}}.
-Proof.
-  iIntros (Φ) "Hl HΦ". iApply twp_lift_atomic_head_step_no_fork; first done.
-  iIntros (σ1 ns κs nt) "(Hσ & Hκs & Hsteps) !>". iDestruct (gen_heap_valid with "Hσ Hl") as %?.
-  iSplit; first by eauto with head_step.
-  iIntros (κ e2 σ2 efs Hstep); inv_head_step.
-  iMod (gen_heap_update with "Hσ Hl") as "[$ Hl]".
-  iMod (steps_auth_update_S with "Hsteps") as "Hsteps".
-  iModIntro. do 2 (iSplit; first done). iFrame. by iApply "HΦ".
-Qed.
-Lemma wp_faa s E l i1 i2 :
-  {{{ ▷ l ↦ LitV (LitInt i1) }}} FAA (Val $ LitV $ LitLoc l) (Val $ LitV $ LitInt i2) @ s; E
-  {{{ RET LitV (LitInt i1); l ↦ LitV (LitInt (i1 + i2)) }}}.
-Proof.
-  iIntros (Φ) ">H HΦ". iApply (twp_wp_step with "HΦ").
-  iApply (twp_faa with "H"); [by auto..|]; iIntros "H HΦ". by iApply "HΦ".
-Qed. *)
+(* TODO: rules to allow splitting the ownership of an array, and having the
+   knowledge of the length of an array be persistent, following what is done in
+   Cosmo. *)
 
 End lifting.
