theories/ml_toy_lang/locoff.v
@@ -1,0 +1,94 @@
+From Coq Require Export ssreflect.
+From stdpp Require Export prelude gmap numbers.
+From iris.heap_lang Require Export locations.
+Set Default Proof Using "Type".
+
+(* A location + offset type, used to look up in the store type where each
+   location is associated to a list of values *)
+
+(* Code adapted from Cosmo https://gitlab.inria.fr/cambium/cosmo
+   (theories/lang/model.v) *)
+
+Notation offset := Z (only parsing).
+Record locoff : Type := Locoff {
+  locoff_loc : loc;
+  locoff_off : offset;
+}.
+
+Definition locoff_to_pair '(Locoff ℓ i) := (ℓ, i).
+Definition pair_to_locoff '(ℓ, i) := Locoff ℓ i.
+Global Instance pair_to_locoff_inj : Inj eq eq pair_to_locoff.
+Proof. by intros [] [] [= -> ->]. Qed.
+Global Instance locoff_to_pair_inj : Inj eq eq locoff_to_pair.
+Proof. by intros [] [] [= -> ->]. Qed.
+Global Instance locoff_eq_dec : EqDecision locoff.
+Proof. eapply (inj_eq_dec locoff_to_pair). Defined.
+Global Instance locoff_countable : Countable locoff.
+Proof. apply (inj_countable' locoff_to_pair pair_to_locoff). by intros []. Qed.
+Definition loc_to_locoff ℓ := Locoff ℓ 0.
+
+Coercion loc_to_locoff : loc >-> locoff.
+Notation "ℓ .[ i ]" := (Locoff ℓ i) (at level 9, format "ℓ .[ i ]").
+
+Section store.
+Context {val : Type}.
+
+Local Notation store := (gmap loc (list val)).
+
+Global Instance store_lookup : Lookup locoff val store :=
+  λ '(Locoff ℓ i) σ,
+    if bool_decide (0 ≤ i)%Z then
+      σ !! ℓ ≫= λ (blk : list _), blk !! Z.to_nat i
+    else None.
+
+Global Instance store_insert : Insert locoff val store :=
+  λ '(Locoff ℓ i) s σ,
+    if bool_decide (0 ≤ i)%Z then
+      match σ !! ℓ with
+      | None     => σ
+      | Some blk => <[ℓ := <[Z.to_nat i := s]> blk]> σ
+      end
+    else σ.
+
+Lemma store_lookup_eq (σ : store) (ℓ : loc) (i : offset) :
+  σ !! ℓ.[i] =
+    if bool_decide (0 ≤ i)%Z then
+      σ !! ℓ ≫= λ (blk : list _), blk !! Z.to_nat i
+    else None.
+Proof. reflexivity. Qed.
+
+Lemma store_lookup_insert (σ : store) (ℓi : locoff) (v0 v : val) :
+  σ !! ℓi = Some v0 →
+  <[ℓi := v]> σ !! ℓi = Some v.
+Proof.
+  destruct ℓi as [ℓ i]. rewrite /lookup /insert /=.
+  case_bool_decide ; last done.
+  case_match ; last done. cbn=>?.
+  rewrite lookup_insert /= list_lookup_insert//. by eapply lookup_lt_Some.
+Qed.
+
+Lemma store_lookup_insert_ne (σ : store) (ℓi ℓi' : locoff) (v : val) :
+  ℓi ≠ ℓi' →
+  <[ℓi := v]> σ !! ℓi' = σ !! ℓi'.
+Proof.
+  destruct ℓi as [ℓ i], ℓi' as [ℓ' i']. rewrite /lookup /insert /=.
+  intros ?. case_bool_decide ; last done.
+  case_bool_decide ; last done.
+  destruct (σ !! ℓ) as [blk|] eqn:Hσℓ ; last done.
+  destruct (decide (ℓ = ℓ')) as [<-|].
+  - destruct (decide (i = i')) as [<-|] ; first done.
+    assert (Z.to_nat i ≠ Z.to_nat i') by lia.
+    by rewrite Hσℓ lookup_insert /= list_lookup_insert_ne.
+  - by rewrite lookup_insert_ne.
+Qed.
+
+Lemma store_insert_offset (σ : store) (ℓ : loc) (i : offset) (vs : list val) (w : val):
+  σ !! ℓ = Some vs →
+  (0 ≤ i < length vs)%Z →
+  <[ℓ.[i] := w]> σ = <[ℓ := <[Z.to_nat i := w]> vs]> σ.
+Proof.
+  intros Hvs Hi. rewrite /insert /store_insert -/(insert _ _ _).
+  case_bool_decide; [|lia]. by simplify_map_eq.
+Qed.
+
+End store.
