theories/ml_toy_lang/notation.v
@@ -21,6 +21,8 @@ Notation LetCtx x e2 := (AppRCtx (LamV x e2)) (only parsing).
 Notation SeqCtx e2 := (LetCtx BAnon e2) (only parsing).
 Notation Match e0 x1 e1 x2 e2 := (Case e0 (Lam x1 e1) (Lam x2 e2)) (only parsing).
 Notation Alloc e := (AllocN (Val $ LitV $ LitInt 1) e) (only parsing).
+Notation Load e := (LoadN e (Val $ LitV $ LitInt 0)) (only parsing).
+Notation Store e e' := (StoreN e (Val $ LitV $ LitInt 0) e') (only parsing).
 
 (* Skip should be atomic, we sometimes open invariants around
    it. Hence, we need to explicitly use LamV instead of e.g., Seq. *)
@@ -71,7 +73,6 @@ Notation "'ref' e" := (Alloc e%E) (at level 10) : expr_scope.
 Notation "- e" := (UnOp MinusUnOp e%E) : expr_scope.
 
 Notation "e1 + e2" := (BinOp PlusOp e1%E e2%E) : expr_scope.
-Notation "e1 +ₗ e2" := (BinOp OffsetOp e1%E e2%E) : expr_scope.
 Notation "e1 - e2" := (BinOp MinusOp e1%E e2%E) : expr_scope.
 Notation "e1 * e2" := (BinOp MultOp e1%E e2%E) : expr_scope.
 Notation "e1 `quot` e2" := (BinOp QuotOp e1%E e2%E) : expr_scope.
